

# 信号处理原理 第 9 次作业

李祥泽 2018011331

由题意

$$e^{-j(n+N)\omega_k} = e^{-jn\omega_k} \cdot e^{-jN\frac{k\cdot 2\pi}{N}} = e^{-jn\omega_k}$$

那么, 欲证等式的右边可如下变换:  $\forall k = 0, 1, 2, 3, \dots, N-1$

$$\begin{aligned} & \sum_{n=0}^{L-1} x(n)e^{-jn\omega_k} \\ &= \sum_{n=0}^{N-1} x(n)e^{-jn\omega_k} + \sum_{n=N}^{2N-1} x(n)e^{-jn\omega_k} + \dots + \sum_{n=rN}^{L-1} x(n)e^{-jn\omega_k} \\ &= \sum_{n=0}^{N-1} x(n)e^{-jn\omega_k} + \sum_{n=0}^{N-1} x(n+N)e^{-j(n+N)\omega_k} + \dots + \sum_{n=0}^{s-1} x(n+rN)e^{-jn\omega_k} \\ & \text{由于序列最后部分补零, 即 } x(n) = 0, n = L, L+1, \dots, N-1+rN \\ &= \sum_{n=0}^{N-1} x(n)e^{-jn\omega_k} + \sum_{n=0}^{N-1} x(n+N)e^{-jn\omega_k} + \dots + \sum_{n=0}^{N-1} x(n+rN)e^{-jn\omega_k} \\ &= \sum_{n=0}^{N-1} \left[ \sum_{m=0}^{r-1} x(n+mN) \right] e^{-jn\omega_k} \\ &= \sum_{n=0}^{N-1} \tilde{x}(n)e^{-jn\omega_k} = \text{等式右边} \end{aligned}$$

即证.